start supporting nat as constants in programs.

src/Verse/Types.v
@@ -73,6 +73,16 @@ Definition Vector256 (t : type direct) := recover (vector 4 t).
 
 Definition constant (ty : type direct) := @typeDenote _ ConstRep direct ty.
 
+Require Verse.Nibble.
+Check Vector.const.
+
+Definition nToConstant (ty : type direct) (n : nat) : constant ty
+  := match ty in type direct return constant ty with
+         | word n => Nibble.fromNat n
+         | multiword m n => Vector.const (Nibble.fromNat n) (2^m)
+         end.
+
+
 Module Type CONST_SEMANTICS (W : WORD_SEMANTICS).
   Parameter constWordDenote : forall n, constant (word n) -> W.wordDenote n.
 End CONST_SEMANTICS.
